git/zaxioms/LeanAlg/LeanAlg/Ffi.lean
@@ -1,34 +1,52 @@
-structure cVec where
-  data : Array Float
+structure genVec (m : Nat) (α : Type u) where
+  data : Fin m -> α 
 
-instance : Inhabited (cVec) where
-  default : cVec := ⟨#[]⟩  
+structure mathVec (m : Nat) where
+  data : Fin m -> Float
 
-namespace cVec
+instance : Inhabited (mathVec m) where
+  default : mathVec m:= ⟨λ _ => 0⟩  
 
-#check cVec.mk
+@[extern "mathVec_initialize"] private constant mathVec_initializer : IO Unit
 
-#check cVec.data
-unsafe def externMk : Array Float -> cVec
-  := panic! "Can't actually do this"
-attribute [implementedBy externMk] cVec.mk
+builtin_initialize mathVec_initializer
+namespace mathVec
 
-unsafe def externData : cVec -> Array Float
-  := panic! "Can't actually do this"
-attribute [implementedBy externData] cVec.data
+@[extern "mathVec_new"]
+def new (m : @&Nat) (x : @&Float) : mathVec m 
+  := ⟨λ m => x⟩  
 
-@[extern "cVec_new"]
-def new (m : @&Nat) (x : @&Float) : cVec 
-  := ⟨mkArray m x⟩  
+-- for whatever reason, when accessing you need to
+-- explicitly type the index such as (3 : Fin a.size)
+@[extern "mathVec_from_array"]
+def from_array (a : @&Array Float) : (mathVec a.size)
+  := ⟨λ i => a[i]⟩  
 
-def from_arr (a : @&Array Float) : cVec
-  := ⟨a⟩  
+@[extern "mathVec_get_val"]
+def get (v : @&mathVec m) (i : @&Fin m) : Float 
+  := v.data i
 
-@[extern "cVec_get_val"]
-def get (v : @&cVec) (i : @&Nat) : Float 
-  := v.data[i]
+@[extern "mathVec_set_val"]
+def set (v : @&mathVec m) (i : @&Fin m) (x : @&Float) : mathVec m
+  := ⟨λ z => if z = i then x else v.data z⟩
 
-@[extern "cVec_dot_prod"]
-def dot_product (v w : @&cVec) : Float
-  := Array.foldr (λ (x, y) z => z + x*y) 0 (Array.zip v.data w.data)
+@[extern "mathVec_scalar_mult"]
+def scalar_multiply (v : @&mathVec m) (s : @& Float) : mathVec m
+  := ⟨λ i => s * v.data i⟩
 
+@[extern "mathVec_add_vector"]
+def add_vector (v w : @&mathVec m) : mathVec m 
+  := ⟨λ i => v.data i + w.data i⟩
+
+-- Supporting functions for Lean
+-- definition of dot product
+def foldl (f : α → β → α) (z : α) : {m : Nat} → (v : genVec m β) → α  
+  | 0, v   => z
+  | m+1, v => foldl f (f z (v.data 0)) ⟨v.data ∘ Fin.succ⟩
+
+def zip (v w : @&mathVec m) : genVec m (Float × Float) 
+  := ⟨λ i => (v.data i, w.data i)⟩ 
+
+@[extern "mathVec_dot_prod"]
+def dot_product (v w : @&mathVec m) : Float
+  := mathVec.foldl (λ z (x, y) => z + (x * y)) 0 (mathVec.zip v w)
