git/zaxioms/LeanAlg/LeanAlg/Main.lean
@@ -4,8 +4,19 @@ import Ffi
 
 def main : IO Unit :=
   do
-    let val := cVec.get (cVec.new 100 100) 99
+    let v1 := mathVec.from_array #[1, 2, 3]
+    let v2 := mathVec.from_array #[2, 2, 9]
+    let add_v1_v2 := @mathVec.add_vector 3 v1 v2
+    let val_add := mathVec.get add_v1_v2 2
+    IO.eprintln (s!"{val_add}")
 
-    let dot := cVec.dot_product (cVec.new 3 5) (cVec.new 3 3)
-    IO.eprintln s!"works"
-    IO.eprintln s!"{dot}"
+    let from_array_val := mathVec.get (mathVec.from_array #[1, 2, 3, 2, 4, 5]) (4 : Fin 6)
+    IO.eprintln (s!"{from_array_val}")
+
+    let mult_val := mathVec.get ((mathVec.from_array #[6, 12, 24]).scalar_multiply 2) (0 : Fin 3)
+    IO.eprintln (s!"{mult_val}")
+
+    let dot_val := @mathVec.dot_product 3 v1 v2
+    IO.eprintln (s!"{dot_val}")
+
+   
